Added the functions mul32, square32 to dettman_multiplication binary

src/PushButtonSynthesis/DettmanMultiplication.v
@@ -55,9 +55,11 @@ Local Coercion QArith_base.inject_Z : Z >-> Q.
 Local Coercion Z.pos : positive >-> Z.
 
 Local Set Keyed Unification. (* needed for making [autorewrite] fast, c.f. COQBUG(https://github.com/coq/coq/issues/9283) *)
-
-Local Opaque reified_mul_gen. (* needed for making [autorewrite] not take a very long time *)
-Local Opaque reified_square_gen. (* needed for making [autorewrite] not take a very long time *)
+(* needed for making [autorewrite] not take a very long time *)
+Local Opaque reified_mul_gen.
+Local Opaque reified_square_gen.
+Local Opaque reified_mul32_gen.
+Local Opaque reified_square32_gen.
 (* needed for making [autorewrite] with [Set Keyed Unification] fast *)
 Local Opaque expr.Interp.
 
@@ -167,7 +169,7 @@ Section __.
          (Some input_bounds, (Some input_bounds, tt))
          (Some output_bounds).
 
- Definition square
+  Definition square
     := Pipeline.BoundsPipeline
          false (* subst01 *)
          possible_values
@@ -177,7 +179,29 @@ Section __.
             @ GallinaReify.Reify n @ GallinaReify.Reify last_limb_width)
          (Some input_bounds, tt)
          (Some output_bounds).
+  
+  Definition mul32
+    := Pipeline.BoundsPipeline
+         false (* subst01 *)
+         possible_values
+         (reified_mul32_gen
+           @ GallinaReify.Reify s @ GallinaReify.Reify c_
+           @ GallinaReify.Reify (Z.to_nat machine_wordsize) @ GallinaReify.Reify n
+           @ GallinaReify.Reify last_limb_width)
+         (Some input_bounds, (Some input_bounds, tt))
+         (Some output_bounds).
 
+  Definition square32
+    := Pipeline.BoundsPipeline
+         false (* subst01 *)
+         possible_values
+         (reified_square32_gen
+            @ GallinaReify.Reify s @ GallinaReify.Reify c_
+            @ GallinaReify.Reify (Z.to_nat machine_wordsize)
+            @ GallinaReify.Reify n @ GallinaReify.Reify last_limb_width)
+         (Some input_bounds, tt)
+         (Some output_bounds).
+ 
   Definition smul (prefix : string)
     : string * (Pipeline.M (Pipeline.ExtendedSynthesisResult _))
     := Eval cbv beta in
@@ -196,25 +220,60 @@ Section __.
            (fun fname : string => [text_before_function_name ++ fname ++ " squares a field element."]%string)
            (square_correct weightf n m input_bounds output_bounds)).
 
+  Definition smul32 (prefix : string)
+    : string * (Pipeline.M (Pipeline.ExtendedSynthesisResult _))
+    := Eval cbv beta in
+        FromPipelineToString!
+          machine_wordsize prefix "mul32" mul32
+          (docstring_with_summary_from_lemma!
+             (fun fname : string => [text_before_function_name ++ fname ++ " multiplies two field elements."]%string)
+             (mul_correct weightf n m input_bounds output_bounds)).
+
+  Definition ssquare32 (prefix : string)
+    : string * (Pipeline.M (Pipeline.ExtendedSynthesisResult _))
+    := Eval cbv beta in
+      FromPipelineToString!
+        machine_wordsize prefix "square32" square32
+        (docstring_with_summary_from_lemma!
+           (fun fname : string => [text_before_function_name ++ fname ++ " squares a field element."]%string)
+           (square_correct weightf n m input_bounds output_bounds)).
+
   (** Work around COQBUG(https://github.com/coq/coq/issues/9286) *)
   Local Opaque DettmanMultiplication.mulmod DettmanMultiplication.squaremod.
+  Local Opaque DettmanMultiplication.mulmod32 DettmanMultiplication.squaremod32.
 
   Local Ltac prove_correctness _ := Primitives.prove_correctness use_curve_good.
 
-  Lemma mul_correct res
+  Lemma mul64_correct res
         (Hres : mul = Success res)
     : mul_correct (weightf) n m input_bounds output_bounds (Interp res).
   Proof using curve_good. prove_correctness (). Qed.
 
-  Lemma Wf_mul res (Hres : mul = Success res) : Wf res.
+  Lemma Wf_mul64 res (Hres : mul = Success res) : Wf res.
   Proof using Type. prove_pipeline_wf (). Qed.
 
-  Lemma square_correct res
+  Lemma square64_correct res
         (Hres : square = Success res)
     : square_correct (weightf) n m input_bounds output_bounds (Interp res).
   Proof using curve_good. prove_correctness (). Qed.
 
-  Lemma Wf_square res (Hres : square = Success res) : Wf res.
+  Lemma Wf_square64 res (Hres : square = Success res) : Wf res.
+  Proof using Type. prove_pipeline_wf (). Qed.
+
+  Lemma mul32_correct res
+        (Hres : mul32 = Success res)
+    : mul_correct (weightf) n m input_bounds output_bounds (Interp res).
+  Proof using curve_good. prove_correctness (). Qed.
+
+  Lemma Wf_mul32 res (Hres : mul32 = Success res) : Wf res.
+  Proof using Type. prove_pipeline_wf (). Qed.
+
+  Lemma square32_correct res
+        (Hres : square32 = Success res)
+    : square_correct (weightf) n m input_bounds output_bounds (Interp res).
+  Proof using curve_good. prove_correctness (). Qed.
+
+  Lemma Wf_square32 res (Hres : square32 = Success res) : Wf res.
   Proof using Type. prove_pipeline_wf (). Qed.
 
   Section for_stringification.
@@ -223,7 +282,9 @@ Section __.
 
     Definition known_functions
       := [("mul", wrap_s smul);
-          ("square", wrap_s ssquare)].
+          ("square", wrap_s ssquare);
+          ("mul32", wrap_s smul32);
+          ("square32", wrap_s ssquare32)].
 
     Definition valid_names : string := Eval compute in String.concat ", " (List.map (@fst _ _) known_functions).
 
@@ -248,10 +309,14 @@ Module Export Hints.
   Hint Opaque
        mul
        square
+       mul32
+       square32
   : wf_op_cache.
 #[global]
   Hint Immediate
-       Wf_mul
-       Wf_square
+       Wf_mul64
+       Wf_square64
+       Wf_mul32
+       Wf_square32
   : wf_op_cache.
 End Hints.
